Kraken/AArch64/Tactics.lean
@@ -1,13 +1,49 @@
 import Kraken.AArch64.Syntax
 import Kraken.AArch64.Semantics
 import Kraken.AArch64.OmniSemantics
+import Kraken.AArch64.Sep
+
+theorem Executable.withAddresses_map_snd (ds : List (Directive × Nat)) (a : Int64) :
+    (Executable.withAddresses (a, ds)).map (·.2) = ds := by
+  induction ds generalizing a with
+  | nil =>
+    unfold Executable.withAddresses
+    rfl
+  | cons d ds ih =>
+    unfold Executable.withAddresses
+    grind
+
+theorem Executable.withAddresses_dropWhile_start (ds : List (Directive × Nat)) (a : Int64) :
+    (Executable.withAddresses (a, ds)).dropWhile (fun x => x.1 ≠ a) =
+      Executable.withAddresses (a, ds) := by
+  cases ds with
+  | nil =>
+    unfold Executable.withAddresses
+    rfl
+  | cons d ds =>
+    unfold Executable.withAddresses
+    simp [List.dropWhile]
+
+theorem Executable.directivesFromStart [layout : Layout] prog :
+    (layout prog).directivesFromAddress layout.start =
+      prog.mapIdx (fun i d => (d, layout.size i)) := by
+  dsimp [Executable.directivesFromAddress, Layout.apply]
+  rw [Executable.withAddresses_dropWhile_start]
+  rw [Executable.withAddresses_map_snd]
+
+macro "kprologue" p:ident : tactic =>
+  `(tactic|
+    (delta $p
+     dsimp only [straightlineStep, Executable.straightline]
+     rw [Executable.directivesFromStart]
+     simp [List.mapIdx, List.mapIdx.go]))
 
 --------------------------------------------------------------------------------
 
 open Lean Meta Sym Sym.DSimp
 open Elab Tactic
 
-partial def peelLambdaLetsAArch64 (f : Expr) (args : Array Expr) (fvars : Array Expr) (k : Expr → Array Expr → DSimpM Result) : DSimpM Result := do
+partial def peelLambdaLets (f : Expr) (args : Array Expr) (fvars : Array Expr) (k : Expr → Array Expr → DSimpM Result) : DSimpM Result := do
   match f with
   | .lam binderName binderType body binderInfo =>
     match body with
@@ -16,39 +52,44 @@ partial def peelLambdaLetsAArch64 (f : Expr) (args : Array Expr) (fvars : Array 
         withLetDecl letName letType letVal fun fvarLet => do
           let instBody : Expr := letBody.instantiate1 fvarLet
           let newLambda := .lam binderName binderType instBody binderInfo
-          peelLambdaLetsAArch64 newLambda args (fvars.push fvarLet) k
+          peelLambdaLets newLambda args (fvars.push fvarLet) k
       else
         k (mkAppN f args) fvars
     | _ => k (mkAppN f args) fvars
   | _ => k (mkAppN f args) fvars
 
-partial def peelLetsAArch64 (e : Expr) (fvars : Array Expr) (k : Expr → Array Expr → DSimpM Result) : DSimpM Result := do
+partial def peelLets (e : Expr) (fvars : Array Expr) (k : Expr → Array Expr → DSimpM Result) : DSimpM Result := do
   match e with
   | .letE name type val body _ =>
     withLetDecl name type val fun fvar =>
-      peelLetsAArch64 (body.instantiate1 fvar) (fvars.push fvar) k
+      peelLets (body.instantiate1 fvar) (fvars.push fvar) k
   | _ =>
     if e.isApp && e.getAppFn.isLambda then
-      peelLambdaLetsAArch64 e.getAppFn e.getAppArgs fvars k
+      peelLambdaLets e.getAppFn e.getAppArgs fvars k
     else
       k e fvars
 
-partial def peelArgsLetsAArch64 (args : Array Expr) (i : Nat) (peeled : Array Expr) (fvars : Array Expr) (k : Array Expr → Array Expr → DSimpM Result) : DSimpM Result := do
+partial def peelArgsLets (args : Array Expr) (i : Nat) (peeled : Array Expr) (fvars : Array Expr) (k : Array Expr → Array Expr → DSimpM Result) : DSimpM Result := do
   if h : i < args.size then
     let arg := args[i]
-    peelLetsAArch64 arg fvars fun arg' fvars' =>
-      peelArgsLetsAArch64 args (i + 1) (peeled.push arg') fvars' k
+    peelLets arg fvars fun arg' fvars' =>
+      peelArgsLets args (i + 1) (peeled.push arg') fvars' k
   else
     k peeled fvars
 
-def kdeltaBetaOnlyAArch64 (targets: List Name) : DSimproc := fun e => do
+def kdeltaBetaOnly (targets: List Name) (maxInstrCount : Option (IO.Ref Nat)) : DSimproc := fun e => do
   unless e.isApp && targets.any e.getAppFn'.isConstOf do return .rfl
 
   let f := e.getAppFn'
   let args := e.getAppArgs
 
-  peelArgsLetsAArch64 args 0 #[] #[] fun (args : Array Expr) (fvars : Array Expr) => do
+  peelArgsLets args 0 #[] #[] fun (args : Array Expr) (fvars : Array Expr) => do
+
     if f.isConstOf ``Effects.All && args[1]!.isApp && args[1]!.getAppFn'.isConstOf ``Directives.interp then
+      if (← maxInstrCount.mapM (·.get)) = .some 0 then
+        return .rfl
+      maxInstrCount.forM (fun r => r.modify (· - 1))
+
       let some arg1 ← Meta.unfoldDefinition? args[1]! true | throwError "can't unfold Directives.interp"
       let e := mkAppN f (args.set! 1 arg1)
       let e' ← shareCommon e
@@ -67,25 +108,31 @@ def kdeltaBetaOnlyAArch64 (targets: List Name) : DSimproc := fun e => do
       else
         return .rfl
 
-def gimmickIdAArch64 (p: Prop): Prop := p
+def gimmickId (p: Prop): Prop := p
 
-def gimmickAArch64 {p: Prop} (h: gimmickIdAArch64 p): p := by
-  simp [gimmickIdAArch64] at h
+theorem gimmick {p: Prop} (h: gimmickId p): p := by
+  simp [gimmickId] at h
   assumption
 
-def gimmickInvAArch64 {p: Prop} (h: p): gimmickIdAArch64 p := by
-  simp [gimmickIdAArch64]
+theorem gimmickInv {p: Prop} (h: p): gimmickId p := by
+  simp [gimmickId]
   assumption
 
-def klogAArch64 : DSimproc := fun e => do
+initialize registerTraceClass `Kraken.kstep
+
+def klog : DSimproc := fun e => do
   let s := (← get).numSteps
-  if e.isApp && e.getAppFn'.isConstOf ``gimmickIdAArch64 then
-    logInfo m!"klog: step {s} visiting\n{e.getAppRevArgs[0]!}"
+  if e.isApp && e.getAppFn'.isConstOf ``gimmickId then
+    trace[Kraken.kstep] "step {s} visiting\n{e.getAppRevArgs[0]!}"
   return .rfl
 
-syntax (name := symKStepAArch64) "kstep_aarch64 " : grind
+structure KStepConfig where
+  debug := false
+declare_term_config_elab elabKStepConfig KStepConfig
 
-def kdsimpMatchAArch64: DSimproc := fun e => do
+syntax (name := symKStep) "kstep" optConfig (ppSpace num)? : grind
+
+def kdsimpMatch: DSimproc := fun e => do
   let some e' ← reduceRecMatcher? e | return .rfl
   let e'' ← Sym.foldProjs e'
   if isSameExpr e e'' then
@@ -93,7 +140,7 @@ def kdsimpMatchAArch64: DSimproc := fun e => do
   else
     return .step (← share e'')
 
-def kbetaAArch64: DSimproc := fun e => do
+def kbeta: DSimproc := fun e => do
   unless e.isApp do return .rfl
   let f := e.getAppFn
   if f.isHeadBetaTargetFn false then
@@ -102,7 +149,7 @@ def kbetaAArch64: DSimproc := fun e => do
   else
     return .rfl
 
-def kdsimpProjAArch64 : DSimproc := fun e => do
+def kdsimpProj : DSimproc := fun e => do
   let f := e.getAppFn
   let .const declName _ := f | return .rfl
   let some _projInfo ← getProjectionFnInfo? declName | return .rfl
@@ -115,48 +162,222 @@ def kdsimpProjAArch64 : DSimproc := fun e => do
       | none   => return .rfl
   reduceProjCont? (← unfoldDefinition? e)
 
-@[grind_tactic symKStepAArch64]
-def evalSymKStepAArch64 : Grind.GrindTactic :=
-  fun _stx : Syntax => do
-  let gGoal : Grind.Goal ← Grind.getMainGoal
-  let mvarId := gGoal.mvarId
+def kLiftLets : DSimproc := fun e => do
+  unless e.isApp && e.getAppFn'.isConstOf ``Effects.All do return .rfl
 
-  let gimmickRule ← mkBackwardRuleFromDecl ``gimmickAArch64
-  let mvarId ← Grind.liftGrindM (do
-    let .goals [mvarId] ← gimmickRule.apply mvarId | failure
-    pure mvarId
-  )
+  let (es, st) ← ExtractLets.extract #[e] |>.run {} |>.run' {} |>.run { givenNames := [] }
+  unless st.decls.size > 0 do return .rfl
 
-  let goal ← mvarId.getType
+  let e' := Meta.ExtractLets.mkLetDecls st.decls es[0]!
+  let e' ← Sym.share e'
+  return .step e'
 
-  let decls := [
-    ``MachineData.setRegOrSp, ``MachineData.setRegOrZr,
-    ``Reg64s.getRegOrSp, ``Reg64s.getRegOrZr, ``Reg64s.setRegOrSp, ``Reg64s.setRegOrZr,
-    ``RegOrSp.base, ``RegOrZr.base,
-    ``Reg64s.getRegOrSp64, ``Reg64s.getRegOrZr64, ``Reg64s.setRegOrSp64, ``Reg64s.setRegOrZr64,
-    ``Reg64s.getXReg, ``Reg64s.setXReg,
-    ``AddrExpr.checkSPAlignment, ``AddrExpr.eval, ``AddrExpr.interp, ``Literal.interp, ``AddrOrLit.interp,
-    ``ExtOrImmReg.interp, ``ShiftRegExpr.interp, ``ExtRegExpr.interp, ``MemExtRegExpr.interp, ``ConstExpr.interp, ``ConstExpr.evalBranchTarget,
-    ``BitVec.apply_extend, ``BitVec.apply_mem_extend,
-    ``Directive.interp, ``Instr.interp, ``Operation.interp,
-    ``Executable.directivesFromAddress, ``Executable.directivesAtAddress, ``Executable.withAddresses, ``Executable.labels,
-    ``Effects.All, ``CondCode.interp, ``StatusFlags.from_result, ``StatusFlags.adds, ``StatusFlags.subs,
-    ``Width.type, ``Width.bits, ``Width.bytes, ``Width.bytesv,
-    ``BitVec.drop, ``BitVec.take, ``BitVec.extractLsb', ``BitVec.truncate
-  ]
+def rwTarget (goal: Grind.Goal) (symm : Bool) (term : Expr) : Grind.GrindTacticM (Grind.Goal × List Grind.Goal) := do
+  goal.withContext do
+    let mvarCounterSaved := (← getMCtx).mvarCounter
+    let r ← Term.withSynthesize do
+      let heq := term
+      let heqType ← instantiateMVars (← inferType heq)
+      let heqType' ← Sym.unfoldReducible heqType
+      let heq ← if isSameExpr heqType heqType' then pure heq else mkExpectedTypeHint heq heqType'
+      goal.mvarId.rewrite (← goal.mvarId.getType) heq symm
+    let mctx ← getMCtx
+    let mvarIds := r.mvarIds.filter fun mvarId => (mctx.getDecl mvarId |>.index) >= mvarCounterSaved
+    let eNew ← Grind.liftSymM <| Sym.preprocessExpr r.eNew
+    let mvarId ← goal.mvarId.replaceTargetEq eNew r.eqProof
+    let mvarIds ← mvarIds.filterM fun mvarId => return !(← mvarId.isAssigned)
+    let sideGoals ← mvarIds.mapM fun mvarId => do
+      let target ← mvarId.getType
+      let target' ← Grind.liftSymM <| Sym.preprocessExpr target
+      if isSameExpr target target' then
+        mvarId.setKind .syntheticOpaque
+        return { goal with mvarId }
+      else
+        let mvarId ← mvarId.replaceTargetDefEq target'
+        return { goal with mvarId }
+    pure ({ goal with mvarId }, sideGoals)
 
-  let goal ← Grind.liftGrindM (do
-    Sym.dsimp
-      (config := { maxSteps := 1000000 })
-      (methods := { pre := klogAArch64 >> kdeltaBetaOnlyAArch64 decls >> kdsimpMatchAArch64 >> kdsimpProjAArch64 >> kbetaAArch64})
-      goal)
+@[grind_tactic symKStep]
+partial def evalSymKStep : Grind.GrindTactic :=
+  fun stx : Syntax => do
+  let cfg := stx[1]
+  let config ← elabKStepConfig cfg
+  let maxSteps? : Option Nat := if stx[2].isNone then none else some stx[2][0].toNat
+  let goal : Grind.Goal ← Grind.getMainGoal
 
-  let mvarId ← mvarId.replaceTargetDefEq goal
+  let gimmickRule ← mkBackwardRuleFromDecl ``gimmick
+  let insertGimmick (goal: Grind.Goal): Grind.GrindTacticM Grind.Goal := do
+    let .goals [mvarId] ← Grind.liftGrindM (gimmickRule.apply goal.mvarId) | failure
+    pure { goal with mvarId }
 
-  let gimmickRule ← mkBackwardRuleFromDecl ``gimmickInvAArch64
-  let mvarId ← Grind.liftGrindM (do
-    let .goals [mvarId] ← gimmickRule.apply mvarId | failure
-    pure mvarId
-  )
+  let gimmickRule ← mkBackwardRuleFromDecl ``gimmickInv
+  let removeGimmick (goal: Grind.Goal): Grind.GrindTacticM Grind.Goal := do
+    let mvarId ← Grind.liftGrindM (do
+      let .goals [mvarId] ← gimmickRule.apply goal.mvarId | failure
+      pure mvarId
+    )
+    pure { goal with mvarId }
 
-  Grind.setGoals [ { gGoal with mvarId } ]
+  let goal ← insertGimmick goal
+  let env ← getEnv
+
+  let declsForDSimp := (kstepExtension.getState env).toList
+  let maxInstrCount ← maxSteps?.mapM (IO.mkRef ·)
+  let kdsimpDecls := kdeltaBetaOnly declsForDSimp maxInstrCount
+
+  let simpTheorems ← ksimpExt.getTheorems
+  let simpMethods: Sym.Simp.Methods := { post := Sym.Simp.evalGround >> simpTheorems.rewrite }
+
+  let specLemmas := (kspecExtension.getState env).toList
+  let specTree: DiscrTree Name ← specLemmas.foldlM (fun specTree name => do
+    let (pat, _) ← mkEqPatternFromDecl name
+    pure (insertPattern specTree pat name)
+  ) {}
+
+  let introsIf (goal: Grind.Goal): Grind.GrindTacticM Grind.Goal := do
+    let goal ← removeGimmick goal
+    let goal ← match ← Grind.liftGrindM (goal.intros #[]) with
+      | Grind.IntrosResult.failed => pure goal
+      | .goal _ goal => pure goal
+    pure (← insertGimmick goal)
+
+  let rec go (goal: Grind.Goal): Grind.GrindTacticM (Grind.Goal × List Grind.Goal) := do
+    let goal ← do
+      let mvarId ← goal.mvarId.replaceTargetDefEq (← Grind.liftGrindM $
+        Sym.dsimp
+          (config := { maxSteps := 1000000 })
+          (methods := {
+            pre := klog >> evalGround >> kdsimpDecls >> kdsimpMatch >> kdsimpProj >> kbeta })
+          (← goal.mvarId.getType))
+      introsIf ({ goal with mvarId })
+
+    if config.debug then
+      let t ← goal.mvarId.getType
+      logInfo m!"MAIN LOOP, after step 1: {goal.mvarId}"
+
+    let (keepGoingSimp, goal) ← Grind.liftGrindM $ do
+      let simpResult ← Sym.simpGoal goal.mvarId simpMethods
+      match simpResult with
+      | .noProgress => pure (false, goal)
+      | .goal mvarId => pure (true, { goal with mvarId })
+      | .closed => throwError "unexpected"
+    if config.debug then
+      let t ← goal.mvarId.getType
+      logInfo m!"MAIN LOOP, after step 2: {t}"
+
+    let goalState ← do
+      let goalT ← goal.mvarId.getType
+      let_expr gimmickId goalT' := goalT | throwError "missing gimmick"
+      let_expr Effects.All post state := goalT' | return (goal, [])
+      pure state
+
+    let (keepGoingSpec, goal) ←
+      match getMatch specTree goalState with
+      | #[ thmName ] =>
+        logInfo m!"Found a spec lemma: {thmName}"
+        let (goal, subGoals) ← rwTarget goal false (mkConst thmName)
+        logInfo m!"{subGoals.length} subgoals generated"
+
+        let subGoals ← subGoals.mapM fun (subGoal: Grind.Goal) => do
+          let simpResult ← Grind.liftGrindM (Sym.simpGoal subGoal.mvarId simpMethods)
+          match simpResult with
+          | .noProgress => pure subGoal
+          | .goal mvarId => pure { subGoal with mvarId }
+          | .closed => pure subGoal
+
+        let solveIfNotAlready: Grind.Goal → Grind.GrindTacticM Bool := fun subGoal => do
+          if ← subGoal.mvarId.isAssigned then
+            let t ← subGoal.mvarId.getType
+            logInfo m!"Already solved: {t}"
+            return false
+
+          if ← withReducible subGoal.mvarId.assumptionCore then
+            let t ← subGoal.mvarId.getType
+            let .some e ← getExprMVarAssignment? subGoal.mvarId | throwError "oh noes"
+            logInfo m!"Solved by exact: {t} by {e}"
+            return true
+
+          try
+            subGoal.mvarId.refl
+            let t ← subGoal.mvarId.getType
+            logInfo m!"Solved by refl: {t}"
+            return true
+          catch _ => pure ()
+
+          try
+            let subGoal ← Grind.liftGrindM subGoal.internalizeAll
+            let t ← subGoal.mvarId.getType
+            match ← Grind.liftGrindM subGoal.grind with
+            | .closed =>
+                logInfo m!"Solved by grind: {t}"
+                return true
+            | .failed _ =>
+                logInfo m!"NOT solved by grind: {t}"
+                throwError "catch me"
+          catch _ =>
+            return false
+
+        let starGoal ← subGoals.findM? (fun g => do
+          let t ← g.mvarId.getType
+          if t.getAppFn.isConstOf ``Std.ExtHashMap.sep then
+            logInfo m!"Found sep goal: {t}"
+            return true
+          else
+            return false
+        )
+
+        if let some g := starGoal then
+          let solved ← solveIfNotAlready g
+          if not solved then
+            return (goal, subGoals)
+
+        while ← (
+          subGoals.foldlM (fun progress subGoal => do
+            let r ← solveIfNotAlready subGoal
+            pure (r || progress)
+          ) false
+        ) do pure ()
+
+        let unsolvedGoals ← subGoals.filterMapM fun (g: Grind.Goal) => do
+          if ← g.mvarId.isAssigned then
+            return none
+          else
+            return some g
+        unsolvedGoals.forM fun mvarId => do
+          let t ← mvarId.mvarId.getType
+          logInfo m!"Unsolved goal: {t}"
+        if unsolvedGoals.length > 0 then
+          return (goal, unsolvedGoals)
+
+        pure (true, goal)
+      | #[] =>
+        pure (false, goal)
+      | _ =>
+        throwError "TODO"
+
+    logInfo m!"kstep: keepGoing = {keepGoingSimp}"
+
+    if keepGoingSimp || keepGoingSpec then
+      go goal
+    else
+      pure (goal, [])
+
+  let (goal, subGoals) ← go goal
+  let goal ← removeGimmick goal
+  
+  logInfo m!"END KSTEP: {subGoals.length} sub-goals left"
+
+  if let .some r := maxInstrCount then
+    let remaining ← r.get
+    if remaining > 0 then
+      throwError m!"kstep could not step through the remaining {remaining} steps"
+
+  Grind.setGoals (subGoals ++ [ goal ])
+
+syntax (name := symRotateRight) "rotate_right" (ppSpace num)? : grind
+
+@[grind_tactic symRotateRight]
+def evalSymRotateRight : Grind.GrindTactic := fun stx => do
+  let n := if stx[1].isNone then 1 else stx[1][0].toNat
+  let goals ← Grind.getGoals
+  Grind.setGoals (goals.rotateRight n)
