KrakenAArch64.lean
@@ -5,6 +5,9 @@
 -/
 
 import Kraken.AArch64.Semantics
+import Kraken.AArch64.OmniSemantics
+import Kraken.AArch64.Sep
+import Kraken.AArch64.Tactics
 import Kraken.AArch64.Parser
 import Kraken.AArch64.Tactics
 import Kraken.AArch64.Sep
